Sum_Util.thy
@@ -1,5 +1,5 @@
 (* Title:  Sum_Util.thy
-   Author: Akama Hitoshi
+   Author: Minamide Yasuhiko, Akama Hitoshi
 *)
 
 theory Sum_Util
@@ -17,5 +17,23 @@ fun inl_list :: "'a \<Rightarrow> ('a + 'b) list" where
 fun inr_list :: "'b \<Rightarrow> ('a + 'b) list" where
   "inr_list y = [Inr y]"
 
+lemma ext_sum:
+  assumes "\<And>l. f (Inl l) = g (Inl l)"
+  assumes "\<And>r. f (Inr r) = g (Inr r)"
+  shows "f = g"
+proof
+  fix x
+  show "f x = g x" using assms by (cases x, simp_all)
+qed
+
+
+lemma map_sum_comp: "map_sum (f1 o f2) (g1 o g2) = map_sum f1 g1 \<circ> map_sum f2 g2"
+  by (rule ext_sum, simp_all)
+
+lemma fold_sum_comp: "fold_sum (f1 o g1) (f2 o g2) = fold_sum f1 f2 o map_sum g1 g2"
+  by (rule ext_sum, simp_all)
+
+lemma map_sum_eq_fold_sum: "map_sum f g = fold_sum (Inl o f) (Inr o g)"
+  by (rule ext_sum, simp_all)
 
 end
